iExploit Tactics

examples/knot/KnotHeader.v
@@ -7,11 +7,154 @@ Require Import Skeleton.
 Require Import PCM.
 Require Import HoareDef.
 Require Import TODOYJ.
-Require Import Logic.
+Require Import Logic YPM.
 
 Generalizable Variables E R A B C X Y Σ.
 
 Set Implicit Arguments.
+
+
+
+
+
+Ltac iIntros :=
+  i;
+  match goal with
+  | |- Impure ?P =>
+    let A := fresh "A" in
+    iIntro A; clear A; iIntros
+  | |- iHyp (Wand ?P _) _ =>
+    let A := fresh "A" in
+    iIntro A; iIntros
+  | |- iHyp (@Univ _ ?X ?P) _ =>
+    let x := fresh "x" in
+    intros x; rewrite intro_iHyp; iIntros
+  | _ => idtac
+  end.
+
+Ltac iAssertP' P H :=
+  let name := fresh "my_r" in
+  pose (name := @URA.unit (@GRA.to_URA _));
+  assert (H: P);
+  [subst name|
+   change P with (iHyp ⌜P⌝ name) in H;
+   on_gwf ltac:(fun GWF => rewrite <- (@URA.unit_id_ _ name eq_refl) in GWF; clearbody name)
+  ]
+.
+
+Tactic Notation "iAssertP" constr(P) :=
+  let H := fresh "H" in
+  iAssertP' P H.
+
+Tactic Notation "iAssertP" constr(P) "as" ident(H) :=
+  iAssertP' P H.
+
+Ltac _iExploit H :=
+  try (match type of H with
+       | iHyp (Wand (Pure ?P) _) _ =>
+         let H0 := fresh "H" in
+         iAssertP P as H0;
+         [auto|iSpecialize H H0; _iExploit H]
+       | iHyp (Wand ?P _) _ =>
+         match goal with
+         | H0:iHyp P _ |- _ =>
+           iSpecialize H H0; _iExploit H
+         end
+       end).
+
+Ltac iExploit H :=
+  match type of H with
+  | iHyp _ _ => _iExploit H
+  | _ =>
+    let T := fresh "T" in
+    hexploit H; intros T; iImpure T; _iExploit T
+  end.
+
+Ltac _puregoal H :=
+  match H with
+  | Wand _ ?Q => _puregoal Q
+  | Pure ?P => constr:(Some P: option Prop)
+  | _ => constr:(None: option Prop)
+  end.
+
+Ltac puregoal H :=
+  match type of H with
+  | iHyp ?H _ => _puregoal H
+  end.
+
+Ltac _iExploitP H :=
+  match (puregoal H) with
+  | Some ?P => cut P; cycle 1; [_iExploit H; try by apply H|]
+  | None => fail
+  end.
+
+Ltac iExploitP H :=
+  match type of H with
+  | iHyp _ _ => _iExploitP H
+  | _ =>
+    let T := fresh "T" in
+    hexploit H; intros T; iImpure T; _iExploitP T
+  end.
+
+Ltac iLeft := left; iRefresh.
+Ltac iRight := right; iRefresh.
+
+
+Definition invRA: URA.t := Auth.t (Excl.t unit).
+Definition inv_black : (@URA.car invRA) := Auth.black (M:=(Excl.t unit)) (Some tt).
+Definition inv_white : (@URA.car invRA) := Auth.white (M:=(Excl.t unit)) (Some tt).
+
+Section AUX.
+  Context `{Σ: GRA.t}.
+  Context `{@GRA.inG invRA Σ}.
+
+  Definition inv_open: iProp := Own (GRA.embed inv_black).
+  Definition inv_closed: iProp := Own (GRA.embed inv_white).
+
+  Lemma inv_closed_unique
+    :
+      ⌞inv_closed -* inv_closed -* ⌜False⌝⌟
+  .
+  Proof.
+    iIntros.
+    unfold inv_closed, inv_white in *.
+    iMerge A A0. rewrite <- own_sep in A. rewrite GRA.embed_add in A.
+    iOwnWf A. eapply GRA.embed_wf in WF. des. repeat ur in WF. ss.
+  Qed.
+
+  Lemma inv_open_unique
+    :
+      ⌞inv_open -* inv_open -* ⌜False⌝⌟
+  .
+  Proof.
+    iIntros.
+    unfold inv_open, inv_black in *.
+    iMerge A A0. rewrite <- own_sep in A. rewrite GRA.embed_add in A.
+    iOwnWf A. eapply GRA.embed_wf in WF. des. repeat ur in WF. ss.
+  Qed.
+End AUX.
+
+Ltac inv_clear :=
+  exfalso; iRefresh;
+  match goal with
+  | H0:iHyp inv_closed _ |- _ =>
+    iExploitP inv_closed_unique; ss
+  | H0:iHyp inv_open _ |- _ =>
+    iExploitP inv_open_unique; ss
+  end; fail.
+
+Section TEST.
+  Context `{Σ: GRA.t}.
+  Context `{@GRA.inG invRA Σ}.
+
+  Goal forall mm,
+      ⌞inv_open -* ⌜mm⌝ -* (⌜mm⌝ -* inv_open) -* ⌜False⌝⌟
+  .
+  Proof.
+    iIntros. red. red.
+    iExploit A1. inv_clear.
+  Qed.
+End TEST.
 
 
 
